Stripped Kernel off

src/dafny/Kernel.dfy
@@ -1,9 +1,0 @@
-class Kernel{
-
-    method exec(instruction:string) {
-        print "Executing instruction " + instruction + " in kernel\n";
-    }
-
-    constructor () {
-    }
-}
